wip closure

src/matroid/flat.lean
@@ -189,6 +189,57 @@ begin
   exact (lt_add_one _).not_le h, 
 end  
 
+lemma indep.not_mem_cl_iff (hI : M.indep I) : 
+  x ∉ M.cl I ↔ x ∉ I ∧ M.indep (insert x I) :=  
+sorry 
+
+lemma indep_of_cl_diff_ne_forall (h : ∀ x ∈ I, M.cl (I \ {x}) ≠ M.cl I) :
+  M.indep I :=
+begin
+  sorry, 
+end 
+   
+lemma mem_cl_iff_exists_basis : 
+  e ∈ M.cl X ↔ ∃ I, M.basis I X ∧ M.basis I (insert e X) :=  
+begin
+  rw mem_cl, sorry, 
+end 
+
+lemma mem_cl_iff_forall_basis : 
+  e ∈ M.cl X ↔ ∀ I, M.basis I X ↔ M.basis I (insert e X) :=  
+begin
+  rw mem_cl, sorry, 
+end 
+
+lemma not_mem_cl_of_basis (hI : M.basis I X) (hI' : ¬M.basis I (insert e X)) :
+  e ∉ M.cl X :=
+sorry 
+
+lemma basis_iff_not_mem_cl :
+  e ∉ M.cl X ↔ e ∉ X ∧ ∃ I, M.basis I X ∧ M.indep (insert e I) := 
+sorry 
+
+
+lemma not_mem_cl_iff_exists_base : 
+  e ∉ M.cl X ↔ e ∉ X ∧ ∃ B, M.base B ∧ e ∈ B ∧ ∀ B', M.base B' → B ∩ X ⊆ B' ∩ X → B' ∩ X = B ∩ X :=     
+begin
+  split, 
+  { sorry},
+  rintros ⟨heX, ⟨B, hB, heB, hBmax⟩⟩ he, 
+  obtain ⟨I, hIBX, hI⟩ := (hB.indep.inter_right X).subset_basis_of_subset (inter_subset_right _ _),  
+  obtain ⟨B',hB', hIB'⟩ := hI.indep,   
+  have := (hBmax _ hB' (hIBX.trans (subset_inter hIB' hI.subset))), 
+  
+  -- rw mem_cl_iff_forall_basis.mp he at hI, 
+  -- have hei : M.indep {e} := hB.indep.subset (by simpa), 
+  -- obtain ⟨I, heI, ⟨B',hB',hIB'⟩, h⟩ := hei.subset_basis_of_subset (subset_union_left {e} X), 
+  
+
+  
+
+
+end 
+
 lemma circuit.subset_cl_diff_singleton (hC : M.circuit C) (e : E) :
   C ⊆ M.cl (C \ {e}) :=
 begin
@@ -203,3 +254,148 @@ begin
 end 
 
 end matroid 
+
+section from_axioms 
+
+/-- A function satisfying the closure axioms determines a matroid -/
+def matroid_of_cl (cl : set E → set E) 
+  (subset_cl : ∀ X, X ⊆ cl X )
+  (cl_mono : ∀ X Y, X ⊆ Y → cl X ⊆ cl Y )
+  (cl_idem : ∀ X, cl (cl X) = cl X )
+  (cl_exchange : ∀ X e f, f ∈ cl (insert e X) \ cl X → e ∈ cl (insert f X) \ cl X ) : 
+matroid E := 
+{ base := λ B, cl B = univ ∧ ∀ X ⊂ B, cl X ≠ univ,
+  exists_base' := 
+  let ⟨B,hB,hBmin⟩ := finite.exists_minimal (λ B, cl B = univ) 
+      ⟨univ, eq_univ_of_univ_subset (subset_cl _)⟩ in 
+    ⟨B, hB, λ X hXB hX, hXB.ne.symm (hBmin _ hX hXB.subset)⟩,
+  base_exchange' := 
+  begin
+    intros B₁ B₂ hB₁ hB₂ x hx, 
+    by_contra' h, 
+    have h₁ : ∀ y ∈ B₂, y ∉ cl (B₁ \ {x}) → cl (insert y (B₁ \ {x})) = univ,
+    { refine λ y hyB₂ hynotin, _, 
+      have hex := cl_exchange (B₁ \ {x}) x y, 
+      rw [insert_diff_singleton, insert_eq_of_mem hx.1, hB₁.1, ←compl_eq_univ_diff, 
+        mem_compl_iff] at hex, 
+      have h' := insert_subset.mpr ⟨(hex hynotin).1, (subset_insert _ _).trans (subset_cl _)⟩,   
+      rw [insert_diff_singleton, insert_eq_of_mem hx.1] at h', 
+      have h'' := cl_mono _ _ h',
+      rwa [cl_idem, hB₁.1, univ_subset_iff] at h''},
+
+    have hss : B₂ \ B₁ ⊆ cl (B₁ \ {x}), 
+    { refine λ y hy, by_contra (λ h', _), 
+      have hxy : x ≠ y, 
+      { rintro rfl, exact hx.2 hy.1},  
+      obtain ⟨A,⟨hAs,hA⟩,hAmin⟩ := finite.exists_minimal _ (h y hy (h₁ y hy.1 h')), 
+      have hxA : x ∉ A, 
+      { refine λ hxA, hxy _,  have := hAs.subset, simpa using this hxA},
+      have hyA : y ∈ A, 
+      { by_contra hyA, 
+        exact hB₁.2 _ (((subset_insert_iff_of_not_mem hyA).mp hAs.subset).trans_ssubset 
+          (diff_singleton_ssubset hx.1)) hA},
+      have hy' : B₁ ⊆ cl (A \ {y}), 
+      { refine λ z hz, by_contra (λ hz', _ ), 
+        have hzA : z ∈ cl (insert y (A \ {y})),
+        { rw [insert_diff_singleton, insert_eq_of_mem hyA, hA], exact mem_univ _,},
+        have h' := (cl_exchange _ _ _ ⟨hzA,hz'⟩).1,
+        have h'' := insert_subset.mpr ⟨h', (subset_insert _ _).trans (subset_cl _)⟩,  
+        rw [insert_diff_singleton, insert_eq_of_mem hyA] at h'',
+        have h''' := cl_mono _ _ h'', 
+        rw [hA, univ_subset_iff, cl_idem] at h''', 
+        refine hB₁.2 _ _ h''', 
+        refine ssubset_of_ne_of_subset _ (insert_subset.mpr ⟨hz,_⟩),
+        { obtain (rfl | hxz) := eq_or_ne x z, 
+          { intro h_eq, 
+            rw [←h_eq, insert_diff_singleton_comm hxy.symm] at hAs, 
+            refine hAs.not_subset _, 
+            rw [diff_subset_iff, insert_comm, singleton_union, insert_diff_singleton, 
+              insert_eq_of_mem hyA], },
+          simp_rw [ne.def, ext_iff, not_forall, mem_insert_iff, mem_diff, mem_singleton_iff], 
+          use x,
+          have := hx.1, tauto},
+        rw [diff_subset_iff, singleton_union], 
+        exact hAs.subset.trans (insert_subset_insert (diff_subset _ _))},
+      have hA' := cl_mono _ _ hy', 
+      rw [hB₁.1, univ_subset_iff, cl_idem] at hA', 
+      refine (diff_singleton_ssubset hyA).ne.symm (hAmin _ ⟨_,hA'⟩ (diff_subset _ _)), 
+      exact (diff_subset _ _).trans_ssubset hAs},
+   
+  have ht : B₂ ⊆ _ := subset_trans _ (union_subset hss (subset_cl (B₁ \ {x}))),  
+  { have ht' := cl_mono _ _ ht, 
+    rw [hB₂.1, cl_idem, univ_subset_iff] at ht', 
+    exact hB₁.2 _ (diff_singleton_ssubset hx.1) ht'},
+  nth_rewrite 0 [←diff_union_inter B₂ B₁], 
+  apply union_subset_union rfl.subset, 
+  rintros y ⟨hy2,hy1⟩, 
+  rw mem_diff_singleton, 
+  use hy1, 
+  rintro rfl, 
+  exact hx.2 hy2, 
+  end }
+
+@[simp] lemma matroid_of_cl_apply (cl : set E → set E) 
+  (subset_cl : ∀ X, X ⊆ cl X )
+  (cl_mono : ∀ X Y, X ⊆ Y → cl X ⊆ cl Y )
+  (cl_idem : ∀ X, cl (cl X) = cl X )
+  (cl_exchange : ∀ X e f, f ∈ cl (insert e X) \ cl X → e ∈ cl (insert f X) \ cl X ) : 
+(matroid_of_cl cl subset_cl cl_mono cl_idem cl_exchange).cl = cl :=
+begin
+
+  -- rw [←not_iff_not], 
+  set M := matroid_of_cl cl subset_cl cl_mono cl_idem cl_exchange with hM, 
+  apply funext, 
+  by_contra' h, 
+  obtain ⟨I,hI,hImin⟩ := finite.exists_minimal _ h,  
+  have hI' : M.indep I, 
+  { apply matroid.indep_of_cl_diff_ne_forall,
+    by_contra' hI', 
+    obtain ⟨x,hxI,hx⟩ := hI', 
+    rw ←hx at hI, 
+    have h' : M.cl (I \ {x}) = cl (I \ {x}), sorry, 
+    apply hI, 
+    refine subset_antisymm _ (hI _).elim,
+    { rw h', apply cl_mono _ _ (diff_subset _ _),  }, 
+    rw h' at hI,  
+    have h'' := M.subset_cl I hxI, 
+    rw [←hx, h'] at h'',  
+    have hi' := insert_subset.mpr ⟨h'', subset_cl _⟩,  
+    rw [insert_diff_singleton, insert_eq_of_mem hxI] at hi', 
+    have hi'' := cl_mono _ _ hi', 
+    rw [cl_idem] at hi'', 
+    rw [hi''.antisymm (cl_mono _ _ (diff_subset _ _)), h']},
+
+  simp_rw [set.ext_iff, not_forall, not_iff, hI'.not_mem_cl_iff, 
+    matroid.indep_iff_subset_base, hM, matroid_of_cl] at hI, 
+  obtain ⟨x,hx⟩ := hI,
+  obtain hxI' | hxI' := em (x ∈ cl I), 
+  { rw [(iff_true _).mpr hxI', iff_true] at hx, 
+    obtain ⟨hxI, B', ⟨hB', hB'min⟩, hIxB'⟩ := hx,   
+      
+    apply hB'min _ (diff_singleton_ssubset (hIxB' (mem_insert x _))), 
+    have hI' : I ⊆ B' \ {x}, 
+      from subset_diff_singleton ((subset_insert _ _).trans hIxB') hxI,   
+    have hx'' : x ∈ cl (B' \ {x}), 
+      from cl_mono _ _ hI' hxI', 
+    have hins := insert_subset.mpr ⟨hx'', subset_cl _⟩,  
+    rw [insert_diff_singleton] at hins, 
+    have hlast := cl_mono _ _ ((subset_insert _ B').trans hins), 
+    rwa [hB', cl_idem, univ_subset_iff] at hlast},
+  have h' := mt hx.1 hxI', 
+  -- rw ←false_iff at hxI', 
+  
+  -- obtain ⟨B, ⟨hB, hBmax⟩, hIB⟩ := hI'
+  simp_rw [not_and, not_exists, ne.def, not_and, and_imp] at h',  
+  obtain ⟨B, hB, hBmin⟩ := finite.exists_minimal (λ B, insert x I ⊆ B ∧ cl B = univ) sorry,
+  refine h' (λ hxI, hxI' (subset_cl I hxI)) _ hB.2 (λ X hXB hXcl, hXB.ne.symm _) hB.1, 
+  -- apply hBmin, 
+  
+  
+
+  
+
+
+  
+end 
+
+end from_axioms
