src/matroid/scratch.lean
@@ -1,27 +1,11 @@
--- import tactic 
+import tactic 
 
--- variables {E : Type*} {P Q : Prop} {e : E}
+open_locale classical 
 
--- example {hP : P ∨ Q} {hQ : ¬P} : Q := by {library_search, }
+variables {E : Type*} {P Q : Prop} {e : E}
 
-import data.finite.card
-
-variables {α : Type*} {s t : set α}
-
-open set
-
-/-- A tactic that finds a `t.finite` term for a set `t` in a `finite` type. -/
-meta def to_finite_tac : tactic unit := `[apply set.to_finite]
-
-/-- Cardinality -/
-noncomputable def set.ncard (s : set α) := nat.card s
-
-
-@[simp] lemma ncard_eq_zero (hs : s.finite . to_finite_tac) :
-  s.ncard = 0 ↔ s = ∅ :=
-sorry
-
-example (ht : t.finite) (hst : s ⊆ t) (hs : s.ncard = 0) : s = ∅  :=
+example {hP : P ↔ Q} {hQ : ¬Q} : ¬P := 
 begin
-  have := λ h, ncard_eq_zero h,
-end
+  have := mt, 
+end 
+
